Account link

CoqOfRust/pinocchio/links/account_info.v
@@ -1,6 +1,6 @@
 Require Import CoqOfRust.CoqOfRust.
 Require Import CoqOfRust.links.M.
-
+Require Import pinocchio.links.pubkey.
 Require Import pinocchio.account_info.
 
 Module Account.
@@ -9,9 +9,90 @@ Module Account.
         is_signer: U8.t;
         is_writable: U8.t;
         executable: U8.t;
-    (* key: Pubkey, *)
-    (* owner: Pubkey, *)
+        key: Pubkey.t;
+        owner: Pubkey.t;
         lamports: U64.t;
         data_len: U64.t
     }.
+
+    Global Instance IsLink : Link t := {
+        Φ := Ty.path "pinocchio::account_info::Account";
+        φ x :=
+      Value.StructRecord "pinocchio::account_info::Account" [] [] [
+        ("borrow_state", φ x.(borrow_state));
+        ("is_signer", φ x.(is_signer));
+        ("is_writable", φ x.(is_writable));
+        ("executable", φ x.(executable));
+        ("key", φ x.(key));
+        ("owner", φ x.(owner));
+        ("lamports", φ x.(lamports));
+        ("data_len", φ x.(data_len))
+      ];
+    }.
+
+    Definition of_ty : OfTy.t (Ty.path "pinocchio::account_info::Account").
+    Proof. eapply OfTy.Make with (A := t); reflexivity. Defined.
+    Smpl Add apply of_ty : of_ty.
+
+    Lemma of_value_with
+    (borrow_state : U8.t) (borrow_state' : Value.t)
+    (is_signer : U8.t) (is_signer' : Value.t)
+    (is_writable : U8.t) (is_writable' : Value.t)
+    (executable : U8.t) (executable' : Value.t)
+    (key : Pubkey.t) (key' : Value.t)
+    (owner : Pubkey.t) (owner' : Value.t)
+    (lamports : U64.t) (lamports' : Value.t)
+    (data_len : U64.t) (data_len' : Value.t)
+    :
+    borrow_state' = φ borrow_state ->
+    is_signer' = φ is_signer ->
+    is_writable' = φ is_writable ->
+    executable' = φ executable ->
+    key' = φ key ->
+    owner' = φ owner ->
+    lamports' = φ lamports ->
+    data_len' = φ data_len ->
+    Value.StructRecord "pinocchio::account_info::Account" [] [] [
+      ("borrow_state", borrow_state');
+      ("is_signer", is_signer');
+      ("is_writable", is_writable');
+      ("executable", executable');
+      ("key", key');
+      ("owner", owner');
+      ("lamports", lamports');
+      ("data_len", data_len')
+    ] = φ (Build_t borrow_state is_signer is_writable executable key owner lamports data_len).
+  Proof. intros; subst; reflexivity. Qed.
+  Smpl Add apply of_value_with : of_value.
+
+  Definition of_value
+    (borrow_state : U8.t) (borrow_state' : Value.t)
+    (is_signer : U8.t) (is_signer' : Value.t)
+    (is_writable : U8.t) (is_writable' : Value.t)
+    (executable : U8.t) (executable' : Value.t)
+    (key : Pubkey.t) (key' : Value.t)
+    (owner : Pubkey.t) (owner' : Value.t)
+    (lamports : U64.t) (lamports' : Value.t)
+    (data_len : U64.t) (data_len' : Value.t):
+    borrow_state' = φ borrow_state ->
+    is_signer' = φ is_signer ->
+    is_writable' = φ is_writable ->
+    executable' = φ executable ->
+    key' = φ key ->
+    owner' = φ owner ->
+    lamports' = φ lamports ->
+    data_len' = φ data_len ->
+    OfValue.t (
+      Value.StructRecord "pinocchio::account_info::Account" [] [] [
+        ("borrow_state", borrow_state');
+        ("is_signer", is_signer');
+        ("is_writable", is_writable');
+        ("executable", executable');
+        ("key", key');
+        ("owner", owner');
+        ("lamports", lamports');
+        ("data_len", data_len')
+      ]).
+  Proof. econstructor; apply of_value_with; eassumption. Defined.
+  Smpl Add apply of_value : of_value.
 End Account.
